theories/utils_array.v
@@ -3,8 +3,128 @@ Require Import ssreflect.
 Require Import ZArith Array.PArray List Floats Lia.
 Import ListNotations.
 
-Require Import Malfunction.Malfunction Malfunction.SemanticsSpec.
+Require Import Malfunction.Malfunction.
 From Coq Require Import Uint63.
+
+Definition int_to_nat (i : int) : nat :=
+  Z.to_nat (Int63.to_Z i).
+
+Definition int_of_nat n := Uint63.of_Z (Coq.ZArith.BinInt.Z.of_nat n).
+
+Lemma int_of_to_nat i :
+  int_of_nat (int_to_nat i) = i.
+Proof.
+  unfold int_of_nat, int_to_nat.
+  rewrite Z2Nat.id.
+  1:eapply Int63.to_Z_bounded.
+  now rewrite Int63.of_to_Z.
+Qed.
+
+Lemma int_to_of_nat i :
+  (Z.of_nat i < Int63.wB)%Z ->
+  int_to_nat (int_of_nat i) = i.
+Proof.
+  unfold int_of_nat, int_to_nat.
+  intros ?.
+  rewrite Int63.of_Z_spec.
+  rewrite Z.mod_small. 1:lia.
+  now rewrite Nat2Z.id.
+Qed.
+
+Lemma wb_max_length :
+  int_to_nat max_length < Z.to_nat Int63.wB.
+Proof.
+  cbn. lia.
+Qed.
+
+Arguments Int63.wB : simpl never.
+Arguments max_length : simpl never.
+
+Ltac lia_max_length := 
+  pose proof wb_max_length; unfold max_length in*; cbn in *; lia.
+
+Module List. 
+  Fixpoint mapi_ {A B} (f : nat -> A -> B) (l : list A) (n:nat) : list B :=
+    match l with
+      | [] => []
+      | x :: l' =>  f n x :: mapi_ f l' (S n) 
+    end.
+
+  Definition mapi {A B} (f : nat -> A -> B) l := mapi_ f l 0. 
+
+  Definition init {A} (size : nat) (f : nat -> A) : list A := map f (seq 0 size).
+
+  Fixpoint set {A} (l : list A) (n : nat) (a:A) : list A 
+   := match l , n with
+     [] , _ =>  []
+   | x :: l , 0 => a :: l
+   | x :: l , S n => x :: set l n a
+   end.
+
+  Lemma length_set A (l : list  A) n a : 
+   List.length (set l n a) = List.length l.
+  Proof. 
+   revert n. induction l; destruct n; cbn; eauto.
+  Qed.
+
+  Lemma nth_set_same A (l : list A) n a d :
+    (n < List.length l) -> nth n (set l n a) d = a.
+  Proof. 
+    revert n. induction l; destruct n; cbn ; intros; try solve [inversion H]; eauto. 
+    apply IHl. now apply Nat.succ_lt_mono in H.
+  Qed. 
+
+  Lemma nth_set_other A (l : list A) n m a d : 
+  n <> m -> nth m (set l n a) d = nth m l d.
+  Proof. 
+   revert n m; induction l; intros; cbn; eauto.
+   destruct n; destruct m; cbn; try congruence.
+   eapply IHl; eauto.  
+  Qed. 
+
+End List. 
+
+Definition Forall2Array {A B:Type} (R : A -> B -> Prop) 
+  (l:list A) (a:array B) default := 
+    List.length l = int_to_nat (PArray.length a) /\
+    forall i:int, int_to_nat i < List.length l -> R (nth (int_to_nat i) l default ) a.[i].
+
+Inductive
+  Forall2_acc {X A B : Type} (R : X -> A -> X -> B -> Prop) : X -> list A -> X -> list B -> Prop :=
+    Forall2_acc_nil : forall x, Forall2_acc R x [] x []
+    | Forall2_acc_cons : forall (x y z : X) (a : A) (b : B) 
+                            (l : list A) (l' : list B) ,
+                     R x a y b -> Forall2_acc R y l z l' -> Forall2_acc R x (a :: l) z (b :: l').
+    
+Fixpoint map_acc {A B S: Type} (f : S -> A -> S * B) (s:S) (l : list A) : S * list B :=
+  match l with
+  | [] => (s , [])
+  | a :: t => let (s',b) := f s a in 
+              let (s'',bs) := map_acc f s' t in (s'', b :: bs)
+  end.
+
+Lemma Forall2_acc_map {S S' A B B'} (R : S -> S' -> Prop) (RB : B -> B' -> Prop)
+        (f : S' -> A -> S' * B') (P : S -> A -> S -> B -> Prop) x x' y l1 l2 :
+  Forall2_acc P x l1 y l2 ->
+  (forall x x' a b y, R x x' -> P x a y b -> let (y' , b') := f x' a in R y y' /\ RB b b') ->
+  R x x' -> 
+  let (y' , l') := map_acc f x' l1 in R y y' /\ Forall2 RB l2 l'.
+Proof.
+  intros H H'. revert x'. induction H; cbn; intros x' Hx; f_equal; eauto.
+  specialize (H' _ _ _ _ _ Hx H). destruct (f _ _ ) as (s',b').
+  destruct H'. specialize (IHForall2_acc _ H1). destruct (map_acc _ _ _).
+  destruct IHForall2_acc. split; eauto.  
+Qed.
+
+Lemma Forall2_acc_length {X A B R x l y l'} : @Forall2_acc X A B R x l y l' -> List.length l = List.length l'.
+Proof. 
+  induction 1; cbn; eauto.
+Qed.   
+
+Lemma Forall2_length {A B P l l'} : @Forall2 A B P l l' -> List.length l = List.length l'.
+Proof. 
+  induction 1; cbn; eauto.
+Qed.
 
 Fixpoint Array_of_List' {A} count (l : list A) (a : array A) :=
   match l with
@@ -97,7 +217,6 @@ Proof.
     eapply nth_indep. lia.
 Qed.
 
-
 Lemma Array_of_list_get_again {A : Set} i s (l : list A) a :
   i >= s + List.length l ->
   s + List.length l < Z.to_nat Int63.wB ->
@@ -124,7 +243,6 @@ Proof.
       * subst. cbn in Hi. lia.
 Qed.
 
-
 Lemma Array_of_list_S A default n a (l:list A) : 
   n < Datatypes.length l ->
   S (Datatypes.length l) <= int_to_nat max_length ->
@@ -132,7 +250,7 @@ Lemma Array_of_list_S A default n a (l:list A) :
   (Array_of_list default l).[int_of_nat n].
 Proof.
   intros. 
-  repeat rewrite Array_of_list_get; cbn in *; try lia; eauto.
+  repeat rewrite Array_of_list_get; try lia_max_length. eauto.
 Qed.
 
 Lemma Array_of_list'_length A k (l:list A) a :
@@ -151,7 +269,57 @@ Proof.
   unfold Array_of_list. rewrite Array_of_list'_length.
   rewrite PArray.length_make. intro H. 
   assert (Hl: (int_of_nat (Datatypes.length l) ≤? max_length)%uint63 = true).
-  { apply leb_spec. rewrite Int63.of_Z_spec. rewrite Z.mod_small; [cbn in *; lia |].
-    cbn in *; lia. }
-  rewrite Hl. apply int_to_of_nat. cbn in *; lia. 
+  { apply leb_spec. rewrite Int63.of_Z_spec. 
+    rewrite Z.mod_small; lia_max_length. }
+  rewrite Hl. apply int_to_of_nat. lia_max_length. 
 Qed.
+
+Lemma Forall2Array_init {A B:Type} (R : A -> B -> Prop) n f g
+   default :
+   n < int_to_nat max_length ->
+   (forall k, k < n ->  R (f k) (g (int_of_nat k))) ->
+   Forall2Array R (List.init n f) (Array_init (int_of_nat n) g) default.
+Proof.
+  intros Hmax HR. unfold Forall2Array.
+  assert (HwB : (Z.of_nat n < Int63.wB)%Z).
+  { clear -Hmax; lia_max_length. }
+  rewrite Array_of_list_length. 
+  { rewrite map_length seq_length. epose (int_to_of_nat n). 
+    unfold int_to_nat in e. now rewrite e. }
+  repeat rewrite map_length seq_length. split; [symmetry; apply int_to_of_nat|]; eauto.
+  intros i Hi. pose (HR (int_to_nat i) Hi). 
+  unfold Array_init. rewrite <- (int_of_to_nat i). 
+  rewrite Array_of_list_get; try lia.
+  1-3: rewrite map_length seq_length; pose (e := int_to_of_nat n HwB);
+       unfold int_to_nat in e; rewrite e; lia.
+  rewrite int_of_to_nat. unfold List.init.  
+  set (k := int_to_nat i) in *. clearbody k; clear i.
+  rewrite map_nth. erewrite nth_indep. erewrite map_nth.
+  pose (int_to_of_nat n HwB). 
+  unfold int_to_nat in e. rewrite e. apply HR. rewrite seq_nth; lia.
+  rewrite map_length seq_length; lia.
+Qed. 
+
+Lemma Forall2Array_cst {A B:Type} (R : A -> B -> Prop) n v v'
+   default :
+   n <= int_to_nat max_length ->
+   R v v' ->
+   Forall2Array R (List.init n (fun _ => v)) (make (int_of_nat n) v') default.
+Proof. 
+  intros Hmax HR. unfold Forall2Array.    
+  repeat rewrite map_length seq_length PArray.length_make.
+  case_eq (int_of_nat n ≤? max_length)%uint63.
+  - split; [symmetry; apply int_to_of_nat|]; eauto.
+    lia_max_length. 
+    intros i Hi. rewrite get_make.
+    set (k := int_to_nat i) in *. unfold List.init.
+    clearbody k; clear i. erewrite nth_indep.
+    erewrite map_nth. Unshelve. 3: exact 0.   exact HR.
+    now rewrite map_length seq_length.
+  - intro abs. pose (leb_spec (int_of_nat n) (max_length)). destruct i. 
+    rewrite H0 in abs.
+    rewrite Int63.of_Z_spec. rewrite Z.mod_small; clear H H0; lia_max_length.
+    inversion abs.
+Qed.     
+
+
